whole bunch of progress! :D

Reflection/Terms.lean
@@ -8,7 +8,7 @@ set_option linter.unusedVariables false
 -- set_option pp.fieldNotation.generalized false
 
 -- move to own util file later:
-@[aesop safe, simp] theorem Fin.add_val_pull {n : Fin (N + 1)} : n < N -> @Fin.val (N + 1) (n + 1) = (@Fin.val (N + 1) n) + 1 := by
+@[aesop unsafe, simp] theorem Fin.add_val_pull {n : Fin (N + 1)} : n < N -> @Fin.val (N + 1) (n + 1) = (@Fin.val (N + 1) n) + 1 := by
   intro h
   rw [Fin.val_add_one_of_lt]
   simp only [Nat.succ_eq_add_one, implies_true]
@@ -16,99 +16,99 @@ set_option linter.unusedVariables false
 
 mutual
   @[aesop unsafe]
-  inductive ECon : Type
-  | nil : ECon
-  | ext : ECon -> ETy -> ECon
+  inductive ConE : Type
+  | nil : ConE
+  | ext : ConE -> TyE -> ConE
   deriving Repr, Inhabited
 
   /-- `Ty : Con -> Type` -/
   @[aesop unsafe]
-  inductive ETy : Type
+  inductive TyE : Type
   /-- `U Γ : Ty Γ` -/
-  | U : ECon -> ETy
+  | U : ConE -> TyE
   /-- `El {Γ} : (t : Tm Γ U) -> Ty Γ` -/
-  | El : ECon -> ETm -> ETy
+  | El : ConE -> TmE -> TyE
   /-- `Pi {Γ} : (A : Ty Γ) -> (B : Ty (Γ, A)) -> Ty Γ` -/
-  | Pi : (Γ : ECon) -> (A : ETy) -> (B : ETy) -> ETy
+  | Pi : (Γ : ConE) -> (A : TyE) -> (B : TyE) -> TyE
   deriving Repr, Inhabited
 
   /-- `Var : (Γ : Con) -> Ty Γ -> Type` -/
   @[aesop unsafe]
-  inductive EVar : Type
+  inductive VarE : Type
   /-- `vz {Γ} {A : Ty Γ} : Var (Γ, A) A[wki]`, note that `wki : (Γ, A) <- Γ`, and `@wki Γ A = wkn (Γ, A) 1`, and `wki = wk id`. -/
-  | vz : (Γ : ECon) -> (A : ETy) -> EVar
+  | vz : (Γ : ConE) -> (A : TyE) -> VarE
   /-- `vs {Γ} ~~{A : Ty Γ}~~ {B : Ty Γ} : Var Γ A -> Var (Γ, B) A[wki]`, but note that `wki` is a shorthand for `wkn (Γ, B) 1 : (Γ, B) <- Γ` -/
-  | vs : (Γ : ECon) -> (B : ETy) -> EVar -> EVar
+  | vs : (Γ : ConE) -> (B : TyE) -> VarE -> VarE
   deriving Repr, Inhabited
 
   /-- `Tm : (Γ : Con) -> Ty Γ -> Type` -/
   @[aesop unsafe]
-  inductive ETm : Type
+  inductive TmE : Type
   /-- `var {Γ} ~~{A : Ty Γ}~~ : Var Γ A -> Tm Γ A` -/
-  | var : (Γ : ECon) -> EVar -> ETm
+  | var : (Γ : ConE) -> VarE -> TmE
   /-- `app {Γ : Con} {A : Ty Γ} {B : Ty (Γ, A)} : (f : Tm Γ (Pi A B)) -> (a : Tm Γ A) -> Tm Γ B[id, a]`.\
     Note that the substitution `(id, a) : Γ <- (Γ, A)` intuitively instantiates de-Brujin variable #0 with `a : Tm Γ A`.  -/
-  | app : (Γ : ECon) -> (A : ETy) -> (B : ETy) -> (f : ETm) -> (a : ETm) -> ETm
+  | app : (Γ : ConE) -> (A : TyE) -> (B : TyE) -> (f : TmE) -> (a : TmE) -> TmE
   /-- `lam {Γ} {A : Ty Γ} {B : Ty (Γ, A)} : (body : Tm (Γ, A) B) -> Tm Γ (Pi A B)` -/
-  | lam : (Γ : ECon) -> (A : ETy) -> (B : ETy) -> (body : ETm) -> ETm
+  | lam : (Γ : ConE) -> (A : TyE) -> (B : TyE) -> (body : TmE) -> TmE
   /-- Only necessary because of substVarE. Will be proven impossible in the final IIRT. -/
-  | error : ETm
+  | error : TmE
   deriving Repr, Inhabited
 
   /-- A substitution `σ : Γ <- Δ` maps every variable in `Δ` to a `Γ`-term.
     Intuitively, it is a list of length `Δ.length` storing terms typed in context `Γ`. -/
   @[aesop unsafe]
-  inductive ESubst : Type
+  inductive SubstE : Type
   /-- `Subst.nil {Γ} : Γ <- ⬝` -/
-  | nil : (Γ : ECon) -> ESubst
+  | nil : (Γ : ConE) -> SubstE
   /-- `Subst.cons {Γ} {Δ} {A : Ty Δ} : (δ : Γ <- Δ) -> (t : Tm Γ A[δ]) -> (Γ <- (Δ, A))` -/
-  | cons : (Γ : ECon) -> (Δ : ECon) -> (A : ETy) -> ESubst -> ETm -> ESubst
+  | cons : (Γ : ConE) -> (Δ : ConE) -> (A : TyE) -> SubstE -> TmE -> SubstE
   deriving Repr, Inhabited
 end
 
-@[aesop unsafe] def ECon.len : ECon -> Nat
+@[aesop unsafe] def ConE.len : ConE -> Nat
 | .nil => 0
 | .ext Γ A => 1 + Γ.len
-notation "∣" Γ:60 "∣" => ECon.len Γ
+notation "∣" Γ:60 "∣" => ConE.len Γ
 
-@[aesop unsafe] def EVar.idxΓ : EVar -> ECon
+@[aesop unsafe] def VarE.idxΓ : VarE -> ConE
 | .vz Γ .. => Γ
 | .vs Γ .. => Γ
 
 /-- Variables are de-Brujin variables. Given `.vs (.vs .vz)`, return `2`. -/
-@[aesop unsafe] def EVar.deBrujin : EVar -> Nat
+@[aesop unsafe] def VarE.deBrujin : VarE -> Nat
 | .vz .. => 0
 | .vs _ _ v => 1 + v.deBrujin
 
 -- This is not provable, because `v.Γ` is arbitrary, since it is not constrained by type indices in the erased version:
--- @[aesop unsafe] theorem EVar.h_val : (v : EVar) -> v.val < ∣v.Γ∣
+-- @[aesop unsafe] theorem VarE.h_val : (v : VarE) -> v.val < ∣v.Γ∣
 -- | .vz .. => ...
 -- | .vs _ _ _ v => ...
 
-@[aesop unsafe] def ESubst.len : ESubst -> Nat
+@[aesop unsafe] def SubstE.len : SubstE -> Nat
 | .nil Γ => 0
 | .cons Γ Δ A σ t => 1 + σ.len
-notation "∣" σ:60 "∣" => ESubst.len σ
-example : ∣ESubst.nil Γ∣ = 0 := ESubst.len.eq_1 Γ -- doesn't work by rfl :(
+notation "∣" σ:60 "∣" => SubstE.len σ
+example : ∣SubstE.nil Γ∣ = 0 := SubstE.len.eq_1 Γ -- doesn't work by rfl :(
 
-@[aesop unsafe] def ESubst.Δ : ESubst -> ECon
+@[aesop unsafe] def SubstE.Δ : SubstE -> ConE
 | .nil Γ => .nil
 | .cons Γ Δ A _ _ => .ext Δ A
-@[aesop unsafe] def ESubst.Γ : ESubst -> ECon
+@[aesop unsafe] def SubstE.Γ : SubstE -> ConE
 | .nil Γ => Γ
 | .cons Γ Δ _ _ _ => Γ
 
 /-- Notation: `Γ ─ n`. Drop the last `n` variables in the context.
   Example: `drop (Con.nil, A, B, C) 1 ≡ (Con.nil, A, B)`. -/
-@[aesop unsafe] def ECon.drop : (Γ : ECon) -> Fin (Γ.len + 1) -> ECon
+@[aesop unsafe] def ConE.drop : (Γ : ConE) -> Fin (Γ.len + 1) -> ConE
 | .nil    , n => .nil
 | .ext Γ A, ⟨0  , h⟩ => .ext Γ A
 | .ext Γ A, ⟨n+1, h⟩ => Γ.drop ⟨n, by rw [len] at h; linarith⟩
-notation Γ:70 " ─ " n:70 => ECon.drop Γ n
+notation Γ:70 " ─ " n:70 => ConE.drop Γ n
 
 /-- Notation: `Γᵥ`. Get the type of the de-Brujin variable `v`.
    `get : (Γ : Con) -> (v : Fin Γ.len) -> Ty (drop Γ (v+1))`. -/
-@[aesop unsafe] def ECon.get : (Γ : ECon) -> (v : Fin Γ.len) -> ETy
+@[aesop unsafe] def ConE.get : (Γ : ConE) -> (v : Fin Γ.len) -> TyE
 | .nil    , v => Fin.elim0 v
 | .ext Γ A, ⟨0  , h⟩ => A
 | .ext Γ A, ⟨v+1, h⟩ => -- expected `Ty (drop (Γ, A) (v+1+1))`
@@ -116,138 +116,16 @@ notation Γ:70 " ─ " n:70 => ECon.drop Γ n
   Γ.get ⟨v, by rw [len] at h; linarith⟩ -- : Ty (drop Γ (v+1))
 
 /-- Substitutions are essentially just lists of terms. So get the term stored at position `v`. -/
-def ESubst.get : (σ : ESubst) -> (v : Fin σ.len) -> ETm
-| .nil Γ, v => Fin.elim0 (ESubst.len.eq_1 _ ▸ v)
+@[aesop unsafe] def SubstE.get : (σ : SubstE) -> (v : Fin σ.len) -> TmE
+| .nil Γ, v => Fin.elim0 (SubstE.len.eq_1 _ ▸ v)
 | .cons _ _ _ σ t, ⟨0  , h⟩ => t
 | .cons _ _ _ σ t, ⟨v+1, h⟩ => σ.get ⟨v, by rw [len] at h; linarith⟩
 
 /-- Look up the term stored in a substitution. -/
-@[aesop unsafe] def substVarE : EVar -> ESubst -> ETm
+@[aesop unsafe] def substVarE : VarE -> SubstE -> TmE
 | .vz _ _  , .cons _ _ _ _ t => t
 | .vs _ _ v, .cons _ _ _ σ _ => substVarE v σ
 | _, _ => .error
-
-section DecreasingMeasure
--- Bodyless definitions. Replace these and theorems about these with `variable`s later.
-variable {substTyE : (Γ Δ : ECon) -> ETy -> ESubst -> ETy}
-variable {substTmE : (Γ Δ : ECon) -> ETm -> ESubst -> ETm}
-variable {wknE : (Γ : ECon) -> (n : Fin (∣Γ∣ + 1)) -> ESubst}
-variable {mkVarE : (Γ : ECon) -> (v : Fin ∣Γ∣) -> EVar}
-variable {compE : (Γ Θ Δ : ECon) -> ESubst -> ESubst -> ESubst}
--- notation A:max"[" σ:max "]" => (substTyE . . A σ)
--- macro:max v:term noWs "[" σ:term "]" : term => `(substVarE $v $σ)
--- macro:max A:term noWs "[" σ:term "]" Γ:term:max Δ:term:max : term => `(substTyE $Γ $Δ $A $σ)
--- macro:max A:term noWs "[" σ:term "]" : term => `(fun x y => substTyE x y $A $σ)
--- macro:max t:term noWs "[" σ:term "]" : term => `(fun x y => substTmE x y $t $σ)
--- notation σ " ∘ " δ => (comp . . . σ δ)
-
--- ## Custom size measure `‖_‖`.
-mutual
-  @[aesop unsafe] def ECon.size : ECon -> Nat
-  | .nil => 1
-  | .ext Γ A => 1 + Γ.size + A.size
-
-  @[aesop unsafe] def ETy.size : ETy -> Nat
-  | .U Δ => 1
-  | .El Δ t => 1 + t.size
-  | .Pi Δ A B => 1 + A.size + B.size
-
-  @[aesop unsafe] def EVar.size : EVar -> Nat
-  | .vz .. => 0
-  | .vs _ _ v => 1 + v.size
-
-  @[aesop unsafe] def ETm.size : ETm -> Nat
-  | .var _ v => 1 + v.size
-  | .app _ _ _ f a => 1 + f.size + a.size
-  | .lam _ _ _ body => 1 + body.size
-  | .error => 0
-
-  @[aesop unsafe] def ESubst.size : ESubst -> Nat
-  | .nil .. => 1
-  | .cons _ _ _ σ t => 1 + σ.size + t.size
-end
-notation "‖" x:60 "‖" => ECon.size x
-notation "‖" x:60 "‖" => ETy.size x
-notation "‖" x:60 "‖" => ETm.size x
-notation "‖" x:60 "‖" => EVar.size x
-notation "‖" x:60 "‖" => ESubst.size x
-
-@[aesop unsafe] theorem ECon.get_lt_con (Γ : ECon) (n : Fin ∣Γ∣) : ‖Γ.get n‖ < ‖Γ‖ := sorry
-@[aesop unsafe] theorem ECon.len_le_sizeOf (Γ : ECon) : ∣Γ∣ <= ‖Γ‖ := sorry
-@[aesop unsafe] theorem ESubst.len_le_sizeOf (σ : ESubst) : ∣σ∣ <= ‖σ‖ := sorry
--- Not provable in the erased version, because type indices not constrained:
--- @[aesop unsafe] theorem ESubst.len_eq_Δ (σ : ESubst) : ∣σ∣ = ∣σ.Δ∣ := sorry
--- @[aesop unsafe] theorem ESubst.len_eq_Δ' (σ : ESubst) : σ.Δ = ΔΔ -> ∣σ∣ = ∣ΔΔ∣ := sorry
-@[aesop unsafe] def ESubst_size (σ : ESubst) : ‖σ‖ = 1 + ∣σ∣ + sum 0 ∣σ∣ (fun v hv => ‖σ.get ⟨v, hv.2⟩‖) := sorry
-
-mutual
-  /-- Counts how many times variable `v` occurs in the type, ignoring type indices. -/
-  def freqTy (Γ : ECon) (v : Fin ∣Γ∣) : ETy -> Nat
-  | .U _ => 0
-  | .El _ t => freqTm Γ v t
-  | .Pi _ A B => freqTy Γ v A + freqTy (.ext Γ A) ⟨v + 1, by rw [ECon.len]; omega⟩ B
-  /-- Counts how many times variable `v` occurs in the term, ignoring type indices. -/
-  def freqTm (Γ : ECon) (v : Fin ∣Γ∣) : ETm -> Nat
-  | .var _ var => if var.deBrujin = v then 1 else 0
-  | .app _ A B f a => freqTm Γ v f + freqTm Γ v a -- ignore type indices A and B
-  | .error => 99999
-  | .lam .. => 99999 -- todo
-end
-
-/-- `(wkn Γ n).size`. Because `wkn (Con.nil, A, B, C) 1 ≡ (Subst.nil, Tm.var #2, Tm.var #1)`,
-  so `1` for `Subst.nil`, and then for every term in the subst we have 1 for `Subst.cons`,
-  1 for `Tm.var`, and `i` for de brujin `#i`. The `i` may not even be necessary actually,
-  making the `sum` needless, but for now I've included `i` just in case. -/
-def wkn.size (Γ : ECon) (n : Fin (Γ.len + 1)) : Nat := 1 + sum n ∣Γ∣ (fun i _ => 2 + i)
-def wknSize (Γlen : Nat) (n : Fin (Γlen + 1)) : Nat := 1 + sum n Γlen (fun i _ => 2 + i)
-@[aesop safe, simp] theorem wkn_size (Γ : ECon) (n : Fin (Γ.len + 1)) : ‖wknE Γ n‖ = wkn.size Γ n := sorry
-
-/-
-  ## cost functions
-  These functions are the "variables" in the system of inequalities below.
--/
-@[simp] noncomputable abbrev substTy? (Γ Δ : ECon) (A : ETy) (σ : ESubst) : Nat := ‖Γ‖ + ‖substTyE Γ Δ A σ‖ + ‖wknE (.ext Γ (substTyE Γ Δ A σ)) 1‖
-@[simp] noncomputable abbrev substTm? (Γ Δ : ECon) (t : ETm) (σ : ESubst) : Nat := 0 -- todo
-@[simp] noncomputable abbrev wkn? (Γ : ECon) (n : Fin (Γ.len + 1)) : Nat := ‖Γ‖ + ∣Γ∣ - n + ‖wknE Γ n‖
-@[simp] noncomputable abbrev mkVar? (Γ : ECon) (v : Fin Γ.len) : Nat := ‖Γ‖ + ‖wknE Γ ⟨v+1, by aesop⟩‖ + v
-@[simp] noncomputable abbrev comp? (Γ Θ Δ : ECon) (δ σ : ESubst) : Nat := ‖δ‖ + ‖σ‖
-
--- ## one theorem per recursive callsite
-
-theorem substTy_1 (t : ETm) (σ : ESubst) : substTm? Γ Δ t σ < @substTy? substTyE wknE Γ Δ (.El Δ t) σ := sorry
-theorem substTy_2 (A B : ETy) (σ : ESubst) : @substTy? substTyE wknE Γ Δ A σ < @substTy? substTyE wknE Γ Δ (.Pi Δ A B) σ := sorry
-theorem substTy_3 (A B : ETy) (σ : ESubst) : @wkn? wknE (.ext Γ (substTyE Γ Δ A σ)) 1 < @substTy? substTyE wknE Γ Δ (.Pi Δ A B) σ := sorry
-theorem substTy_4 (A B : ETy) (σ : ESubst) : comp? (.ext Γ (substTyE Γ Δ A σ)) Γ Δ σ (wknE (.ext Γ (substTyE Γ Δ A σ)) 1) < @substTy? substTyE wknE Γ Δ (.Pi Δ A B) σ := sorry
-theorem substTy_5 (A B : ETy) (σ : ESubst) : @substTy? substTyE wknE (.ext Γ (substTyE Γ Δ A σ)) (.ext Δ A) B (compE (.ext Γ (substTyE Γ Δ A σ)) Γ Δ σ (wknE (.ext Γ (substTyE Γ Δ A σ)) 1)) < @substTy? substTyE wknE Γ Δ (.Pi Δ A B) σ := sorry
-
-theorem substTm_1 (f a : ETm) (σ : ESubst) : substTm? Γ Δ f σ < substTm? Γ Δ (.app Δ A B f a) σ := sorry
-theorem substTm_2 (f a : ETm) (σ : ESubst) : substTm? Γ Δ a σ < substTm? Γ Δ (.app Δ A B f a) σ := sorry
-theorem substTm_3 (f a : ETm) (σ : ESubst) : @wkn? wknE (.ext Γ (substTyE Γ Δ A σ)) 1 < substTm? Γ Δ (.app Δ A B f a) σ := sorry
-theorem substTm_4 (f a : ETm) (σ : ESubst) : comp? (.ext Γ (substTyE Γ Δ A σ)) Γ Δ σ (wknE (.ext Γ (substTyE Γ Δ A σ)) 1) < substTm? Γ Δ (.app Δ A B f a) σ := sorry
-theorem substTm_5 (f a : ETm) (σ : ESubst) : @substTy? substTyE wknE (.ext Γ (substTyE Γ Δ A σ)) (.ext Δ A) B (compE (.ext Γ (substTyE Γ Δ A σ)) Γ Δ σ (wknE (.ext Γ (substTyE Γ Δ A σ)) 1)) < substTm? Γ Δ (.app Δ A B f a) σ := sorry
-
-theorem wkn_1 (Γ : ECon) (n : Fin (Γ.len + 1)) (h : n < Γ.len) : @wkn? wknE Γ (n+1) < @wkn? wknE Γ n := by
-  simp_all only [wkn?, wkn_size, wkn.size, sum_begin]
-  rw [Fin.add_val_pull h]
-  omega
-theorem wkn_2 (Γ : ECon) (n : Fin (Γ.len + 1)) : (h : n < Γ.len) -> @mkVar? wknE Γ ⟨n, sorry⟩ < @wkn? wknE Γ n := sorry
-
-theorem mkVar_1 (Γ : ECon) (v : Fin Γ.len) : @wkn? wknE Γ (v.castAdd 1) < @mkVar? wknE (.ext Γ X) (ECon.len.eq_2 .. ▸ v.natAdd 1) := sorry
-theorem mkVar_2 (Γ : ECon) (v : Fin Γ.len) (h : v + 1 < ∣.ext Γ X∣) :
-  (@substTy? substTyE wknE
-    Γ
-    (Γ.drop ⟨v+1, by rw [ECon.len] at h; linarith⟩)
-    (Γ.get ⟨v, by rw [ECon.len] at h; linarith⟩) -- `Γᵥ`
-    (wknE (.ext Γ X) ⟨v+1+1, by simp_all only [ECon.len, add_lt_add_iff_right]⟩) -- `wkn (Γ, X) (v+1+1)`
-  ) -- `Γᵥ[wkn (Γ, X) (v+1+1)]`
-  < @mkVar? wknE (.ext Γ X) (ECon.len.eq_2 .. ▸ v.natAdd 1)
-  := sorry
-theorem mkVar_3 (Γ : ECon) (v : Fin Γ.len)       : @mkVar? wknE Γ v < @mkVar? wknE (.ext Γ X) (ECon.len.eq_2 .. ▸ v.natAdd 1) := sorry
-
--- not 100% on the rhs of `<` of these two:
-theorem comp_1 (δ σ : ESubst) : comp? Γ Θ Δ δ σ < comp? Γ Θ (.ext Δ A) (.cons Θ Δ A δ t) σ := by sorry
-theorem comp_2 (δ σ : ESubst) : substTm? Γ Θ t σ < comp? Γ Θ (.ext Δ A) (.cons Θ Δ A δ t) σ := sorry
-end DecreasingMeasure
 
 #check Fin.castSucc
 #check Fin.val_add_one_of_lt
@@ -257,11 +135,11 @@ abbrev Fin.addOne (n : Fin (N+1)) (h : n.val < N) : Fin (N+1) := ⟨n.val + 1, b
 
 mutual
   /-- `wkn {Γ : Con} (n : Fin (Γ.len + 1)) : (Γ <- Γ - n)` -/
-  def wknE (Γ : ECon) (n : Fin (Γ.len + 1)) : ESubst :=
+  def wknE (Γ : ConE) (n : Fin (Γ.len + 1)) : SubstE :=
     if h : Γ.len = n then .nil Γ
     else
       have h : n < ∣Γ∣ := by omega
-      ESubst.cons
+      SubstE.cons
         Γ
         (Γ.drop (n.addOne h))
         (Γ.get ⟨n.val, h⟩) -- Γₙ
@@ -273,7 +151,7 @@ mutual
   termination_by Γ.len - n
 
   -- `mkVar : (Γ : Con) -> (v : Fin Γ.len) -> Var Γ (Γ.get v)[wkn Γ (v+1)]`
-  def mkVarE : (Γ : ECon) -> (v : Fin Γ.len) -> EVar
+  def mkVarE : (Γ : ConE) -> (v : Fin Γ.len) -> VarE
   | .nil, v => Fin.elim0 v
   | .ext Γ X, ⟨0  , _⟩ => -- expected `Var (Γ, X) (get (Γ, X) 0)[wkn (Γ, X) (0 + 1)]`
     -- by defeq we have `get (Γ, X) 0 ≡ X`
@@ -285,59 +163,59 @@ mutual
       Γ
       -- (substTyE
       --   Γ
-      --   (Γ.drop ⟨v+1, by rw [ECon.len] at h; linarith⟩)
-      --   (Γ.get ⟨v, by rw [ECon.len] at h; linarith⟩) -- `Γᵥ`
-      --   (wkn (.ext Γ X) ⟨v+1+1, by simp_all only [ECon.len, add_lt_add_iff_right]⟩) -- `wkn (Γ, X) (v+1+1)`
+      --   (Γ.drop ⟨v+1, by rw [ConE.len] at h; linarith⟩)
+      --   (Γ.get ⟨v, by rw [ConE.len] at h; linarith⟩) -- `Γᵥ`
+      --   (wkn (.ext Γ X) ⟨v+1+1, by simp_all only [ConE.len, add_lt_add_iff_right]⟩) -- `wkn (Γ, X) (v+1+1)`
       -- ) -- `Γᵥ[wkn (Γ, X) (v+1+1)]`
       X
-      (mkVarE Γ ⟨v, by rw [ECon.len] at h; linarith⟩) -- `mkVar Γ v : Var Γ (Γ.get v)[wkn Γ (v+1)]`
+      (mkVarE Γ ⟨v, by rw [ConE.len] at h; linarith⟩) -- `mkVar Γ v : Var Γ (Γ.get v)[wkn Γ (v+1)]`
   termination_by Γ v => sizeOf Γ
 end
 
 #print axioms wknE
 
 /-- Identity substitution. `id : {Γ : Con} -> (Γ <- Γ)`. Just a shorthand for `wkn Γ 0`. -/
-def idE (Γ : ECon) : ESubst := wknE Γ 0
+def idE (Γ : ConE) : SubstE := wknE Γ 0
 
 /-- Weakened identity substitution. `wki : {Γ : Con} -> {W : Ty Γ} -> (Γ, W <- Γ)`. Just a shorthand for `wkn (Γ, W) 1`. -/
-def wkiE (Γ : ECon) (W : ETy) : ESubst := wknE (.ext Γ W) 1
+def wkiE (Γ : ConE) (W : TyE) : SubstE := wknE (.ext Γ W) 1
 
 mutual
   /-- `substTy {Γ Δ : Con} (A : Ty Δ) (σ : Γ <- Δ) : Ty Γ` -/
-  unsafe def substTyE (Γ Δ : ECon) : ETy -> ESubst -> ETy
+  unsafe def substTyE (Γ Δ : ConE) : TyE -> SubstE -> TyE
   | .U Δ, σ => .U Γ
   | .El Δ t, σ => .El Γ (substTmE Γ Δ t σ)
   | .Pi Δ A B, σ => -- Δ ⊢ A
-    let Aσ : ETy /- Γ -/ := substTyE Γ Δ A σ -- `Γ ⊢ A[σ]`
+    let Aσ : TyE /- Γ -/ := substTyE Γ Δ A σ -- `Γ ⊢ A[σ]`
     let wk_σ /- : (Γ, A[σ]) <- Δ -/ := compE (.ext Γ Aσ) Γ Δ σ (wknE (.ext Γ Aσ) 1) -- note that `wk σ = σ ∘ (wkn (Γ, A[σ]) 1)`
-    -- let A_wk_σ : ETy := substTyE (.ext Γ Aσ) Δ A wk_σ -- `(Γ, A[σ]) ⊢ A[wk σ]`
-    let vz : ETm /- (Γ, A[σ]) A[wk σ] -/ := .var (.ext Γ Aσ) (.vz Γ Aσ) -- `.vz Γ A' : Var (Γ, A[σ]) A[σ][wk id]`, note that `wk σ = σ ∘ (wk id)`
-    let δ : ESubst /- (Γ, A[σ]) <- (Δ, A) -/ := .cons (.ext Γ Aσ) Δ A (wk_σ) vz
+    -- let A_wk_σ : TyE := substTyE (.ext Γ Aσ) Δ A wk_σ -- `(Γ, A[σ]) ⊢ A[wk σ]`
+    let vz : TmE /- (Γ, A[σ]) A[wk σ] -/ := .var (.ext Γ Aσ) (.vz Γ Aσ) -- `.vz Γ A' : Var (Γ, A[σ]) A[σ][wk id]`, note that `wk σ = σ ∘ (wk id)`
+    let δ : SubstE /- (Γ, A[σ]) <- (Δ, A) -/ := .cons (.ext Γ Aσ) Δ A (wk_σ) vz
     .Pi Γ Aσ (substTyE (.ext Γ Aσ) (.ext Δ A) B δ)
   termination_by A σ => sizeOf A + sizeOf σ
 
   /-- `substTm {Γ Δ : Con} {A : Ty Δ} (t : Tm Δ A) (σ : Subst Γ Δ) : Tm Γ (substTy A σ)` -/
-  unsafe def substTmE (Γ Δ : ECon) : ETm -> ESubst -> ETm
+  unsafe def substTmE (Γ Δ : ConE) : TmE -> SubstE -> TmE
   | .var _ v, σ => substVarE v σ -- just pick the term in the subst that v refers to. if ill-formed, then .error.
   | .app _Δ A B f a, σ => -- `Δ ⊢ a : A`, `Δ ⊢ f : Pi A B`, expected `Tm Γ B[id, a][σ]`    (yes this `A` is the same as the `A` in `@substTm _ _ A ..`)
-    let Aσ : ETy /- Γ -/ := substTyE Γ Δ A σ -- Γ ⊢ A[σ]
-    -- let wk_σ : ESubst := wkE Γ Δ A' σ -- `wk σ : (Γ, A[σ]) <- Δ`, note that `wk σ = σ ∘ (wk id)`
-    let wk_σ : ESubst := compE (.ext Γ Aσ) Γ Δ σ (wknE (.ext Γ Aσ) 1) -- `wk σ : (Γ, A[σ]) <- Δ`, note that `wk σ = σ ∘ (wkn (Γ, A[σ]) 1)`
-    -- let A_wk_σ : ETy /- (Γ, A[σ]) -/ := substTyE (.ext Γ Aσ) Δ A wk_σ -- A[wk σ]
-    let vz : ETm /- (Γ, A[σ]) A[wk σ] -/ := .var (.ext Γ Aσ) (.vz Γ Aσ) -- `.vz Γ A[σ] : Var (Γ, A[σ]) A[σ][wk id]`, note that `wk σ = (wk id) ∘ σ`
-    let δ : ESubst /- (Γ, A[σ]) <- (Δ, A) -/ := ESubst.cons (.ext Γ Aσ) Δ A (wk_σ) vz
+    let Aσ : TyE /- Γ -/ := substTyE Γ Δ A σ -- Γ ⊢ A[σ]
+    -- let wk_σ : SubstE := wkE Γ Δ A' σ -- `wk σ : (Γ, A[σ]) <- Δ`, note that `wk σ = σ ∘ (wk id)`
+    let wk_σ : SubstE := compE (.ext Γ Aσ) Γ Δ σ (wknE (.ext Γ Aσ) 1) -- `wk σ : (Γ, A[σ]) <- Δ`, note that `wk σ = σ ∘ (wkn (Γ, A[σ]) 1)`
+    -- let A_wk_σ : TyE /- (Γ, A[σ]) -/ := substTyE (.ext Γ Aσ) Δ A wk_σ -- A[wk σ]
+    let vz : TmE /- (Γ, A[σ]) A[wk σ] -/ := .var (.ext Γ Aσ) (.vz Γ Aσ) -- `.vz Γ A[σ] : Var (Γ, A[σ]) A[σ][wk id]`, note that `wk σ = (wk id) ∘ σ`
+    let δ : SubstE /- (Γ, A[σ]) <- (Δ, A) -/ := SubstE.cons (.ext Γ Aσ) Δ A (wk_σ) vz
 
-    let B' : ETy := substTyE (.ext Γ Aσ) (.ext Δ A) B δ
-    let f' : ETm := substTmE Γ Δ f σ -- `f[σ] : Tm Γ (Pi A B)[σ]`, where `(Pi A B)[σ] = Pi A[σ] B[wk σ, #0]` per definition of substTy
-    let a' : ETm := substTmE Γ Δ a σ -- `a[σ] : Tm Γ A[σ]`
-    let fa' : ETm := .app Γ Aσ B' f' a' -- `.app f[σ] a[σ] : Tm Γ B[wk σ, #0][id, a]`
+    let B' : TyE := substTyE (.ext Γ Aσ) (.ext Δ A) B δ
+    let f' : TmE := substTmE Γ Δ f σ -- `f[σ] : Tm Γ (Pi A B)[σ]`, where `(Pi A B)[σ] = Pi A[σ] B[wk σ, #0]` per definition of substTy
+    let a' : TmE := substTmE Γ Δ a σ -- `a[σ] : Tm Γ A[σ]`
+    let fa' : TmE := .app Γ Aσ B' f' a' -- `.app f[σ] a[σ] : Tm Γ B[wk σ, #0][id, a]`
     fa' -- ! here we need `((wk σ), #0) ∘ (id, a) = (id, a) ∘ σ` to typecheck.
   | .lam Δ A B body, σ => .error
   | .error, _ => .error
   termination_by t σ => sizeOf t + sizeOf σ
 
   /-- `comp {Γ Θ Δ : Con} : Subst Θ Δ -> Subst Γ Θ -> Subst Γ Δ` -/
-  unsafe def compE (Γ Θ Δ : ECon) : ESubst -> ESubst -> ESubst
+  unsafe def compE (Γ Θ Δ : ConE) : SubstE -> SubstE -> SubstE
   | .nil Θ         , σ => .nil Γ
   | .cons Θ Δ A δ t, σ => -- `δ : Θ <- Δ`,   `σ : Γ <- Θ`,   `Θ ⊢ t : A[δ]`,   expected `Γ <- Δ, A`
     .cons Γ Δ A
@@ -347,21 +225,21 @@ mutual
 end
 
 /-- `wk : {Γ Δ : Con} -> {W : Ty Γ} -> (Γ <- Δ) -> (Γ, W <- Δ)` -/
-unsafe def wkE (Γ Δ : ECon) (W : ETy) (σ : ESubst) : ESubst
+unsafe def wkE (Γ Δ : ConE) (W : TyE) (σ : SubstE) : SubstE
   := compE (.ext Γ W) Γ Δ σ (wkiE Γ W) -- `wki : Γ,W <- Γ`
 
 /-- Parellel weakening `wkp {Γ Δ} {A : Ty Δ} (σ : Γ <- Δ) : (Γ, A[σ]) <- (Δ, A)`. This is the `δ` used in substTyE and substTmE. -/
-unsafe def wkpE (Γ Δ : ECon) (A : ETy) (σ : ESubst) : ESubst :=
-  let Aσ : ETy /- Γ -/ := substTyE Γ Δ A σ -- `Γ ⊢ A[σ]`
-  let wk_σ : ESubst := compE (.ext Γ Aσ) Γ Δ σ (wknE (.ext Γ Aσ) 1) -- `wk σ : (Γ, A[σ]) <- Δ`, note that `wk σ = σ ∘ (wkn (Γ, A[σ]) 1)`
-  let vz : ETm /- (Γ, A[σ]) A[wk σ] -/ := .var (.ext Γ Aσ) (.vz Γ Aσ) -- `.vz Γ A[σ] : Var (Γ, A[σ]) A[σ][wk id]`, note that `wk σ = (wk id) ∘ σ`
-  let δ : ESubst /- (Γ, A[σ]) <- (Δ, A) -/ := ESubst.cons (.ext Γ Aσ) Δ A wk_σ vz
+unsafe def wkpE (Γ Δ : ConE) (A : TyE) (σ : SubstE) : SubstE :=
+  let Aσ : TyE /- Γ -/ := substTyE Γ Δ A σ -- `Γ ⊢ A[σ]`
+  let wk_σ : SubstE := compE (.ext Γ Aσ) Γ Δ σ (wknE (.ext Γ Aσ) 1) -- `wk σ : (Γ, A[σ]) <- Δ`, note that `wk σ = σ ∘ (wkn (Γ, A[σ]) 1)`
+  let vz : TmE /- (Γ, A[σ]) A[wk σ] -/ := .var (.ext Γ Aσ) (.vz Γ Aσ) -- `.vz Γ A[σ] : Var (Γ, A[σ]) A[σ][wk id]`, note that `wk σ = (wk id) ∘ σ`
+  let δ : SubstE /- (Γ, A[σ]) <- (Δ, A) -/ := SubstE.cons (.ext Γ Aσ) Δ A wk_σ vz
   .cons (.ext Γ Aσ) Δ A wk_σ vz
 
 section Tests
-  def F'' : ETy := .Pi (.nil) (.U .nil) (.U .nil)
-  -- def Γ : ECon := (.ext (.ext (.ext .nil (.U .nil)) F) F)
-  def Γe'' : ECon := .ext (.ext (.ext (.ext .nil (.U .nil)) F'') F'') F''
+  def F'' : TyE := .Pi (.nil) (.U .nil) (.U .nil)
+  -- def Γ : ConE := (.ext (.ext (.ext .nil (.U .nil)) F) F)
+  def Γe'' : ConE := .ext (.ext (.ext (.ext .nil (.U .nil)) F'') F'') F''
   #reduce sizeOf <| idE Γe''
   #reduce sizeOf <| wkpE Γe'' Γe'' F'' <| idE Γe''
 
@@ -373,12 +251,12 @@ section Tests
   #eval idE (.ext (.ext .nil (.U .nil)) (.U .nil))
   #eval idE (.ext (.ext (.ext .nil (.U .nil)) (.U .nil)) (.U .nil))
 
-  def wk1 (Γ : ECon) : ESubst := wknE Γ 1
+  def wk1 (Γ : ConE) : SubstE := wknE Γ 1
   #eval wk1 (.ext .nil (.U .nil))
   #eval wk1 (.ext (.ext .nil (.U .nil)) (.U .nil))
   #eval wk1 (.ext (.ext (.ext .nil (.U .nil)) (.U .nil)) (.U .nil))
 
-  def wk2 (Γ : ECon) : ESubst := wknE Γ 2
+  def wk2 (Γ : ConE) : SubstE := wknE Γ 2
   #eval wk2 (.ext (.ext .nil (.U .nil)) (.U .nil))
   #eval wk2 (.ext (.ext (.ext .nil (.U .nil)) (.U .nil)) (.U .nil))
 
@@ -386,8 +264,8 @@ section Tests
 end Tests
 
 
-/-- `def idxA : Var Γ A -> Ty Γ := A`. Reconstruct the `A` in `Var Γ A`. -/
-noncomputable unsafe def EVar.idxA : EVar -> ETy
+/-- `def idxA : Var Γ A -> Ty Γ := A`. RConEstruct the `A` in `Var Γ A`. -/
+noncomputable unsafe def VarE.idxA : VarE -> TyE
 | .vz Γ A => A
 | .vs Γ B v => -- `.vs v : Var (Γ, B) A[wkn (Γ, B) 1]`, and `v : Var A Γ`, and ~~`Γ⊢A`~~, and `Γ,A⊢B`, expecting `Ty (Γ, B)`.
   let A := v.idxA -- `Γ ⊢ A`
@@ -395,37 +273,47 @@ noncomputable unsafe def EVar.idxA : EVar -> ETy
   let A_wk := substTyE Γ (.ext Γ B) A (wknE (.ext Γ B) 1) -- `Γ, B ⊢ A[wkn (Γ, B) 1]`
   A_wk
 
--- /-- Reconstruct the `A` in `Tm Γ A`. -/
--- noncomputable unsafe def ETm.idxA : ETm -> ETy
+-- /-- RConEstruct the `A` in `Tm Γ A`. -/
+-- noncomputable unsafe def TmE.idxA : TmE -> TyE
 -- | .var Γ v => v.idxA
--- | .app Γ A B f a => A -- this is the one spot where we *need* to store `A`. Intuitively, `.app` is modus ponens, so similar to cuts in sequent calculus. We can't do cut elimination in Lean afaik, so we are unable to reconstruct `A` here.
+-- | .app Γ A B f a => A -- this is the one spot where we *need* to store `A`. Intuitively, `.app` is modus ponens, so similar to cuts in sequent calculus. We can't do cut elimination in Lean afaik, so we are unable to rConEstruct `A` here.
 -- | .lam .. => sorry
 -- | .error .. => sorry
 
+#check VarE.idxA
+
 mutual
-  @[aesop safe constructors unsafe cases]
-  unsafe inductive ConW : ECon -> Prop
+  @[aesop unsafe constructors unsafe cases]
+  unsafe inductive ConW : ConE -> Prop
   | nil : ConW .nil
   | ext : (Γw : ConW Γ) -> (Aw : TyW Γ A) -> ConW (.ext Γ A)
 
-  @[aesop safe constructors unsafe cases]
-  unsafe inductive TyW : ECon -> ETy -> Prop
+  @[aesop unsafe constructors unsafe cases]
+  unsafe inductive TyW : ConE -> TyE -> Prop
   | U : ConW Γ -> TyW Γ (.U Γ)
   | El : ConW Γ -> TmW Γ (.U Γ) t -> TyW Γ (.El Γ t)
   | Pi : ConW Γ -> TyW Γ A -> TyW (.ext Γ A) B -> TyW Γ (.Pi Γ A B)
   /-- A mutual inductive type which may refer to existing types in Γ, and has type A. -/
   -- | mind : MInd /- Γ -/ A -> Ty Γ
 
-  @[aesop safe constructors unsafe cases]
-  unsafe inductive VarW : ECon -> ETy -> EVar -> Prop
-  /-`vz {Γ} {A : Ty Γ} : Var (Γ, A) A[wki]` -/
+  -- @[aesop unsafe constructors unsafe cases]
+  -- unsafe inductive VarW : ConE -> TyE -> VarE -> Prop
+  -- /- `vz {Γ} {A : Ty Γ} : Var (Γ, A) A[wki]` -/
+  -- | vz : ConW Γ -> TyW Γ A -> VarW (.ext Γ A) (substTyE (.ext Γ A) Γ A (wkiE Γ A)) (.vz Γ A)
+  -- /- `vs {Γ} ~~{A : Ty Γ}~~ {B : Ty Γ} : Var Γ A -> Var (Γ, B) A[wki]` -/
+  -- | vs : ConW Γ -> TyW Γ A -> TyW Γ B -> VarW Γ A v
+  --   -> VarW (.ext Γ B) (substTyE (.ext Γ B) Γ A (wkiE Γ B)) (.vs Γ /- ~~A~~ -/ B v)
+
+  @[aesop unsafe constructors unsafe cases]
+  unsafe inductive VarW : ConE -> TyE -> VarE -> Prop
+  /- `vz {Γ} {A : Ty Γ} : Var (Γ, A) A[wki]` -/
   | vz : ConW Γ -> TyW Γ A -> VarW (.ext Γ A) (substTyE (.ext Γ A) Γ A (wkiE Γ A)) (.vz Γ A)
   /- `vs {Γ} ~~{A : Ty Γ}~~ {B : Ty Γ} : Var Γ A -> Var (Γ, B) A[wki]` -/
-  | vs : ConW Γ -> TyW Γ A -> TyW Γ B -> VarW Γ A v
+  | vs : ConW Γ -> /-~~ TyW Γ A -> ~~-/ TyW Γ B -> VarW Γ A v
     -> VarW (.ext Γ B) (substTyE (.ext Γ B) Γ A (wkiE Γ B)) (.vs Γ /- ~~A~~ -/ B v)
 
-  @[aesop safe constructors unsafe cases]
-  unsafe inductive TmW : ECon -> ETy -> ETm -> Prop
+  @[aesop unsafe constructors unsafe cases]
+  unsafe inductive TmW : ConE -> TyE -> TmE -> Prop
   /- var {Γ} ~~{A : Ty Γ}~~ : Var Γ A -> Tm Γ A -/
   | var : ConW Γ -> /- ~~ TyW Γ A -> ~~-/ VarW Γ A v -> TmW Γ A (.var Γ /- ~~A~~ -/ v)
   /- `app {Γ : Con} {A : Ty Γ} {B : Ty (Γ, A)} : (f : Tm Γ (Pi A B)) -> (a : Tm Γ A) -> Tm Γ B[id, a]`
@@ -439,8 +327,8 @@ mutual
   --         (bodyw : TmW (.ext Γe Ae) Be bodye) ->
   --         TmW Γe (.Pi Ae Be) (.lam bodye)
 
-  @[aesop safe constructors unsafe cases]
-  unsafe inductive SubstW : ECon -> ECon -> ESubst -> Prop
+  @[aesop unsafe constructors unsafe cases]
+  unsafe inductive SubstW : ConE -> ConE -> SubstE -> Prop
   | nil : ConW Γ -> SubstW Γ .nil (.nil Γ)
   /- Subst.cons {Γ} {Δ} {A : Ty Δ} : (δ : Γ <- Δ) -> (t : Tm Γ A[δ]) -> (Γ <- (Δ, A)) -/
   | cons : ConW Γ -> ConW Δ -> TyW Δ A ->
@@ -449,71 +337,84 @@ mutual
       SubstW Γ (.ext Δ A) (.cons Γ Δ A δ t)
 end
 
-@[simp] theorem Γ_len0_nil {Γ : ECon} {n : Fin (Γ.len + 1)} (h : Γ.len = 0) : Γ = .nil :=
+@[simp] theorem Γ_len0_nil {Γ : ConE} {n : Fin (Γ.len + 1)} (h : Γ.len = 0) : Γ = .nil :=
   match Γ with
   | .nil => rfl
-  | .ext Γ A => by rw [ECon.len] at h; rename_i Γ_1; simp_all only [add_eq_zero, one_ne_zero, false_and]
+  | .ext Γ A => by rw [ConE.len] at h; rename_i Γ_1; simp_all only [add_eq_zero, one_ne_zero, false_and]
 
-@[simp] theorem drop_0' : {Γ : ECon} -> {h : 0 < ∣Γ∣ + 1} -> Γ ─ ⟨0, h⟩ = Γ
+@[simp] theorem drop_0' : {Γ : ConE} -> {h : 0 < ∣Γ∣ + 1} -> Γ ─ ⟨0, h⟩ = Γ
 | .nil    , _ => rfl
-| .ext Γ A, h => ECon.drop.eq_2 Γ A h
+| .ext Γ A, h => ConE.drop.eq_2 Γ A h
 
-@[simp] theorem drop_0 : {Γ : ECon} -> Γ ─ 0 = Γ := drop_0'
+@[simp] theorem drop_0 : {Γ : ConE} -> Γ ─ 0 = Γ := drop_0'
 
-@[simp] theorem drop_ext_1' : {Γ : ECon} -> {h : 1 < ∣Γ.ext A∣ + 1} -> .ext Γ A ─ ⟨1, h⟩ = Γ
-| .nil    , _ => by simp only [ECon.drop, Fin.zero_eta, Fin.isValue, drop_0]
-| .ext Γ A, h => by simp only [ECon.drop, Fin.zero_eta, drop_0]
--- @[simp] theorem drop_ext_1 : {Γ : ECon} -> .ext Γ A ─ 1 = Γ := by aesop
+@[simp] theorem drop_ext_1' : {Γ : ConE} -> {h : 1 < ∣Γ.ext A∣ + 1} -> .ext Γ A ─ ⟨1, h⟩ = Γ
+| .nil    , _ => by simp only [ConE.drop, Fin.zero_eta, Fin.isValue, drop_0]
+| .ext Γ A, h => by simp only [ConE.drop, Fin.zero_eta, drop_0]
+-- @[simp] theorem drop_ext_1 : {Γ : ConE} -> .ext Γ A ─ 1 = Γ := by aesop
 
-@[simp] theorem drop_all {Γ : ECon} {n : Fin (Γ.len + 1)} (h : Γ.len = n) : Γ ─ n = .nil :=
+@[simp] theorem drop_ext_1_n : {Γ : ConE} -> {h : _ < ∣Γ.ext A∣ + 1} -> {h' : _ < _} -> .ext Γ A ─ ⟨n+1, h⟩ = Γ ─ ⟨n, h'⟩
+| .nil    , _ => by simp only [ConE.drop, Fin.zero_eta, Fin.isValue, drop_0]
+| .ext Γ A, h => by simp only [ConE.drop, Fin.zero_eta, drop_0]
+
+@[simp] theorem drop_all {Γ : ConE} {n : Fin (Γ.len + 1)} (h : Γ.len = n) : Γ ─ n = .nil :=
   match Γ, n with
   | Γ, 0 => by
     rw [Γ_len0_nil h, drop_0]
     exact 0 -- this is so weird?
   | .ext Γ A, ⟨.succ n, hsn⟩ => by
-    rw [ECon.drop]
-    exact @drop_all Γ ⟨n, by simp_all only [ECon.len, Nat.succ_eq_add_one]; rw [add_comm, h]; simp⟩
+    rw [ConE.drop]
+    exact @drop_all Γ ⟨n, by simp_all only [ConE.len, Nat.succ_eq_add_one]; rw [add_comm, h]; simp⟩
       (by -- ugly proof
         simp_all only
         simp_all only [Nat.succ_eq_add_one, lt_add_iff_pos_right, zero_lt_one]
-        rw [ECon.len.eq_2] at h
+        rw [ConE.len.eq_2] at h
         omega)
 
-@[simp] theorem wknE_all {Γ : ECon} {n : Fin (Γ.len + 1)} (h : Γ.len = n) : wknE Γ n = .nil Γ := by
+@[simp] theorem wknE_all {Γ : ConE} {n : Fin (Γ.len + 1)} (h : Γ.len = n) : wknE Γ n = .nil Γ := by
   rw [wknE]
   simp only [dite_eq_left_iff, imp_false, Decidable.not_not]
   exact h
 
-@[aesop safe] unsafe def dropW : (Γw : ConW Γ) -> (n : Fin (∣Γ∣+1)) -> ConW (Γ ─ n)
+@[aesop unsafe] unsafe def dropW : (Γw : ConW Γ) -> (n : Fin (∣Γ∣+1)) -> ConW (Γ ─ n)
 | ConW.nil    , n => .nil
 | Γw, ⟨0  , h⟩ => by rw [drop_0']; exact Γw
 | @ConW.ext Γ A Γw Aw, ⟨n+1, h⟩ => by
-  rw [ECon.drop]
-  exact dropW Γw ⟨n, by rw [ECon.len] at h; omega⟩
+  rw [ConE.drop]
+  exact dropW Γw ⟨n, by rw [ConE.len] at h; omega⟩
 
-@[aesop safe] unsafe def getW {Γ : ECon} : (Γw : ConW Γ) -> (v : Fin Γ.len) -> TyW (Γ ─ v.succ) (Γ.get v)
+@[aesop unsafe] unsafe def getW {Γ : ConE} : (Γw : ConW Γ) -> (v : Fin Γ.len) -> TyW (Γ ─ v.succ) (Γ.get v)
 | .nil    , v => Fin.elim0 v
-| @ConW.ext Γ A Γw Aw, ⟨0  , h⟩ => by simp only [Fin.succ_mk, Nat.succ_eq_add_one, zero_add, ECon.drop, drop_0', ECon.get]; exact Aw
-| @ConW.ext Γ A Γw Aw, ⟨v+1, h⟩ => by simp [ECon.drop, ECon.get]; exact getW Γw ⟨v, by rw [ECon.len] at h; omega⟩
+| @ConW.ext Γ A Γw Aw, ⟨0  , h⟩ => by simp only [Fin.succ_mk, Nat.succ_eq_add_one, zero_add, ConE.drop, drop_0', ConE.get]; exact Aw
+| @ConW.ext Γ A Γw Aw, ⟨v+1, h⟩ => by simp [ConE.drop, ConE.get]; exact getW Γw ⟨v, by rw [ConE.len] at h; omega⟩
 
 /-- `(Γ - (v+1), Γᵥ) = Γ - v` -/
 @[simp]
-theorem con_ext_get' (Γ : ECon) (v : Fin Γ.len) (h1 : ↑v + 1 < ∣Γ∣ + 1) (h2 : ↑v < ∣Γ∣) (h' : ↑v < ∣Γ∣ + 1)
-  : .ext (Γ ─ ⟨v+1, h1⟩) (Γ.get ⟨v, h2⟩) = Γ ─ ⟨v, h'⟩
+theorem con_ext_get' (Γ : ConE) (v : Fin Γ.len) (h1 : ↑v + 1 < ∣Γ∣ + 1) (h2 : ↑v < ∣Γ∣) (h' : ↑v < ∣Γ∣ + 1)
+  : .ext (Γ ─ ⟨v+1, h1⟩) (Γ.get ⟨v, h2⟩)    =    Γ ─ ⟨v, h'⟩
   := by
   match Γ, v with
   | .nil    , n => exact Fin.elim0 n
-  | .ext Γ A, ⟨0  , h⟩ => simp only [zero_add, drop_ext_1', ECon.get, Fin.zero_eta, drop_0]
+  | .ext Γ A, ⟨0  , h⟩ => simp only [zero_add, drop_ext_1', ConE.get, Fin.zero_eta, drop_0]
   | .ext Γ A, ⟨v+1, h⟩ =>
-    have ih := con_ext_get' Γ ⟨v, by rw [ECon.len] at h; omega⟩ (by omega) (by omega) (by omega)
-    simp only [ECon.drop, ECon.get, ih]
+    have ih := con_ext_get' Γ ⟨v, by rw [ConE.len] at h; omega⟩ (by omega) (by omega) (by omega)
+    simp only [ConE.drop, ConE.get, ih]
 
--- theorem con_ext_get (Γ : ECon) (v : Fin Γ.len) : .ext (Γ ─ v.succ) (Γ.get v) = Γ ─ v.castSucc := by sorry -- con_ext_get'
+-- theorem con_ext_get (Γ : ConE) (v : Fin Γ.len) : .ext (Γ ─ v.succ) (Γ.get v) = Γ ─ v.castSucc := by sorry -- con_ext_get'
 
+@[simp] theorem get_0 (Γ : ConE) (A : TyE) {h : 0 < ∣Γ.ext A∣} : (Γ.ext A).get ⟨0, h⟩ = A := by rw [ConE.get]
+
+/-- `get (Γ, X) (v+1) = get Γ v` -/
+@[simp] theorem get_ext_1 (Γ : ConE) (A : TyE) (v) {h : _ < _} {h'} : (Γ.ext A).get ⟨v+1, h⟩ = Γ.get ⟨v, h'⟩ := by rw [ConE.get]
+
+-- ! need theorem : wkn Γ (v+1) ∘ wkn (Γ, X) 1 = wkn (Γ, X) (v+1+1)
+
+-- set_option pp.proofs true in
+-- set_option pp.explicit true in
 mutual
   /-- `wkn {Γ : Con} (n : Fin (Γ.len + 1)) : (Γ <- Γ - n)` -/
   unsafe def wknW (Γw : ConW Γ) (n : Fin (Γ.len + 1)) : SubstW Γ (Γ ─ n) (wknE Γ n) := by
-    -- SubstW.nil {Γe : ECon} : ConW Γe → SubstW ECon.nil Γe (ESubst.nil Γe)
+    -- SubstW.nil {Γe : ConE} : ConW Γe → SubstW ConE.nil Γe (SubstE.nil Γe)
     if h : Γ.len = n then
       rw [wknE_all h, drop_all h]
       exact @SubstW.nil Γ Γw
@@ -531,179 +432,112 @@ mutual
           Γw
           (mkVarW Γw ⟨n.val, h⟩)
         )
-      simp [ECon.drop, Fin.addOne] at this
+      simp [ConE.drop, Fin.addOne] at this
       let v : Fin Γ.len := ⟨n, by omega⟩ -- maybe adapting `con_ext_get'` makes more sense than introducing this v
       have rw := con_ext_get' Γ v (by omega) (by omega) (by omega)
       -- have n_is_v : n.val = v.val := by simp_all only [Fin.eta]
       -- rw [n_is_v] at h
       rw [rw] at this
-      clear rw
       rw [wknE]
-      simp [reduceDite] -- why doesn't it simp away the `if` :(
-      -- this almost works, just a bit of fiddling around with Fin
-      exact this
+      simp_all only [Fin.eta, ↓reduceDite]
 
   -- `mkVar : (Γ : Con) -> (v : Fin Γ.len) -> Var Γ Γₙ[wkn Γ (v+1)]`
   unsafe def mkVarW : (Γw : ConW Γ) -> (v : Fin Γ.len) ->
     VarW Γ (substTyE Γ (Γ ─ ⟨v.val + 1, by omega⟩) (Γ.get ⟨v.val, by omega⟩) (wknE Γ v.succ)) (mkVarE Γ v)
   | .nil, v => Fin.elim0 v
-  | @ConW.ext Γe Xe Γw Xw, ⟨0  , h⟩ => by -- expected `Var (Γ, X) (get (Γ, X) 0)[wkn (Γ, X) (0 + 1)]`
+  | @ConW.ext Γ X Γw Xw, ⟨0  , h⟩ => by -- expected `Var (Γ, X) (get (Γ, X) 0)[wkn (Γ, X) (0 + 1)]`
     -- by defeq we have `get (Γ, X) 0 ≡ X`
-    rw [wknE]
     rw [mkVarE]
+    simp [Fin.addOne]
+    have := VarW.vz Γw Xw
+    rw [wkiE] at this
+    -- have rw := @Fin.eta (∣Γ.ext X∣ + 1) 1 (by omega)
+    have h : 1 < ∣Γ.ext X∣ + 1 := by omega
+    have : ⟨1, h⟩ = (1 : Fin (∣Γ.ext X∣ + 1)) := by
+      sorry -- how is this hard lmao
+      done
+    simp_all only [Nat.succ_eq_add_one]
+  | @ConW.ext Γ X Γw Xw, ⟨v+1, h⟩ => by -- expected `Var (Γ, X) (get (Γ, X) (v+1))[wkn (Γ, X) (v + 1 + 1)]`
+    rw [ConE.len] at h
+    -- simp
+    rw [drop_ext_1_n (h := by omega)]
     simp
+    rw [get_ext_1]
 
-    exact .vz Γw Xw -- `: Var (Γ, X) X[wki]`, where `wki` is just a shorthand for `wkn (Γ, X) 1`.
-  | .ext Γ X, ⟨v+1, h⟩ => -- expected `Var (Γ, X) (get (Γ, X) (v+1))[wkn (Γ, X) (v + 1 + 1)]`
-    -- ! need theorem get_ext : get (Γ, X) (v+1) = get Γ v
+    let varr := mkVarE Γ ⟨v, by omega⟩
+    let A := varr.idxA
+
+    have ih := mkVarW Γw ⟨v, by omega⟩
+    simp at ih
+
+    -- ! need theorem : A[σ][δ] = A[σ ∘ δ]
+
     -- ! need theorem : wkn Γ (v+1) ∘ wkn (Γ, X) 1 = wkn (Γ, X) (v+1+1)
-    .vs
-      Γ
-      -- (substTyE
-      --   Γ
-      --   (Γ.drop ⟨v+1, by rw [ECon.len] at h; linarith⟩)
-      --   (Γ.get ⟨v, by rw [ECon.len] at h; linarith⟩) -- `Γᵥ`
-      --   (wkn (.ext Γ X) ⟨v+1+1, by simp_all only [ECon.len, add_lt_add_iff_right]⟩) -- `wkn (Γ, X) (v+1+1)`
-      -- ) -- `Γᵥ[wkn (Γ, X) (v+1+1)]`
-      X
-      (mkVarE Γ ⟨v, by rw [ECon.len] at h; linarith⟩) -- `mkVar Γ v : Var Γ (Γ.get v)[wkn Γ (v+1)]`
-  -- termination_by Γ v => sizeOf Γ
+    --                  ^^^^^^^^^^^^^^^^^^^^^^^^^^                         this is (part of) the resulting type we get from `Var.vs`
+    --                                               ^^^^^^^^^^^^^^^^^^    this is (part of) the expected type for this match arm.
+
+    -- TODO finish this proof
+    /- VarW.vs {Γ : ConE} {~~A~~ B : TyE} {v : VarE} : ConW Γ → TyW Γ A → TyW Γ B → VarW Γ A v → VarW (Γ.ext B) (substTyE (Γ.ext B) Γ A (wkiE Γ B)) (VarE.vs Γ B v)-/
+    have := VarW.vs (A := varr.idxA) Γw /-~~ A[wki] ~~-/ Xw ih
+    -- exact this
+    done
 end
 
+-- TODO:
+mutual
+  /-- `substTy {Γ Δ : Con} (A : Ty Δ) (σ : Subst Γ Δ) : Ty Γ` -/
+  unsafe def substTyW (Γw : ConW Γ) (Δw : ConW Δ) (Aw : TyW Δ A) (σw : SubstW Γ Δ σ) : TyW Γ (substTyE Γ Δ A σ) := sorry
+  /-- `substTm {Γ Δ : Con} {A : Ty Δ} (t : Tm Δ A) (σ : Subst Γ Δ) : Tm Γ (substTy A σ)` -/
+  unsafe def substTmW (Γw : ConW Γ) (Δw : ConW Δ) (Aw : TyW Δ A) (tw : TmW Δ A t) (σw : SubstW Γ Δ σ) : TmW Γ (substTyE Γ Δ A σ) (substTmE Γ Δ t σ) := sorry
+  /-- `comp {Γ Θ Δ : Con} : Subst Θ Δ -> Subst Γ Θ -> Subst Γ Δ` -/
+  unsafe def compW (Γw : ConW Γ) (Θw : ConW Θ) (Δw : ConW Δ) (δw : SubstW Θ Δ δ) (σw : SubstW Γ Θ σ) : SubstW Γ Δ (compE Γ Θ Δ δ σ) := sorry
+end
 
+unsafe def Con : Type                                                                               := @PSigma ConE ConW
+unsafe def Ty (Γ : Con) : Type                                                                      := @PSigma TyE (TyW Γ.1)
+unsafe def Var (Γ : Con) (A : Ty Γ) : Type                                                          := @PSigma VarE (VarW Γ.1 A.1)
+unsafe def Tm (Γ : Con) (A : Ty Γ) : Type                                                           := @PSigma TmE (TmW Γ.1 A.1)
+unsafe def Subst (Γ Δ : Con) : Type                                                                 := @PSigma SubstE (SubstW Γ.1 Δ.1)
+
+unsafe def Con.len (Γ : Con) : Nat                                                                  := Γ.1.len
+unsafe def Con.drop (Γ : Con) (n : Fin (Γ.len + 1)) : Con                                           := ⟨Γ.1.drop n, dropW Γ.2 n⟩
+unsafe def Con.get (Γ : Con) (v : Fin Γ.len) : Ty (Γ.drop v.succ)                                   := ⟨Γ.1.get v, getW Γ.2 v⟩
+unsafe def wkn {Γ : Con} (n : Fin (Γ.len + 1)) : Subst Γ (Γ.drop n)                                 := ⟨wknE Γ.1 n, wknW Γ.2 n⟩
+unsafe def substTy {Γ Δ : Con} (A : Ty Δ) (σ : Subst Γ Δ) : Ty Γ                                    := ⟨substTyE Γ.1 Δ.1 A.1 σ.1, substTyW Γ.2 Δ.2 A.2 σ.2⟩
+unsafe def substTm {Γ Δ : Con} {A : Ty Δ} (t : Tm Δ A) (σ : Subst Γ Δ) : Tm Γ (substTy A σ)         := ⟨substTmE Γ.1 Δ.1     t.1 σ.1, substTmW Γ.2 Δ.2 A.2 t.2 σ.2⟩
+unsafe def comp {Γ Θ Δ : Con} (δ : Subst Θ Δ) (σ : Subst Γ Θ) : Subst Γ Δ                           := ⟨compE Γ.1 Θ.1 Δ.1 δ.1 σ.1, compW Γ.2 Θ.2 Δ.2 δ.2 σ.2⟩
+/-- `mkVar : (Γ : Con) -> (v : Fin Γ.len) -> Var Γ  Γᵥ[wkn Γ (v+1)]` -/
+unsafe def mkVar {Γ : Con} (v : Fin Γ.len) : Var Γ (substTy (Γ.get v) (wkn v.succ))                 := ⟨mkVarE Γ.1 v, mkVarW Γ.2 v⟩
+
+unsafe def Con.nil : Con                                                                            := ⟨.nil, .nil⟩
+unsafe def Con.ext (Γ : Con) (A : Ty Γ) : Con                                                       := ⟨.ext Γ.fst A.fst, .ext Γ.snd A.snd⟩
+unsafe def Ty.U : Ty Γ                                                                              := ⟨.U Γ.1, .U Γ.2⟩
+unsafe def Ty.El (t : Tm Γ .U) : Ty Γ                                                               := ⟨.El Γ.1 t.fst, .El Γ.2 t.snd⟩
+unsafe def Ty.Pi (A : Ty Γ) (B : Ty (.ext Γ A)) : Ty Γ                                              := ⟨.Pi Γ.1 A.fst B.fst, .Pi Γ.2 A.snd B.snd⟩
+
+-- TODO: rest of the constructors (easy)
+-- /-- `vz {Γ} {A : Ty Γ} : Var (Γ, A) A[wki]`, note that `wki : (Γ, A) <- Γ`, and `@wki Γ A = wkn (Γ, A) 1`, and `wki = wk id`. -/
+-- unsafe def Var.vz : Var (Con.ext Γ A) (substTy A wk) := ⟨.vz Γ.1 A.1, .vz Γ.2 A.2⟩
+-- /-- `vs {Γ} ~~{A : Ty Γ}~~ {B : Ty Γ} : Var Γ A -> Var (Γ, B) A[wki]`, but note that `wki` is a shorthand for `wkn (Γ, B) 1 : (Γ, B) <- Γ` -/
+-- unsafe def Var.vs (v : Var Γ A) : Var (Con.ext Γ B) (substTy A wk) := ⟨.vs v.fst, .vs v.snd⟩
+-- unsafe def Subst.nil : Subst Γ Con.nil := ⟨.nil, .nil⟩
+-- unsafe def Subst.cons (δ : Subst Γ Δ) (t : Tm Γ (substTy A δ)) : Subst Γ (Con.ext Δ A) := ⟨.cons δ.fst t.fst, .cons δ.snd t.snd⟩
+-- unsafe def Tm.app {A : Ty Γ} {B : Ty (Con.ext Γ A)} (f : Tm Γ (Ty.Pi A B)) (a : Tm Γ A) : Tm Γ (substTy B (subst1 a)) -- Tm Γ B[Var.vz ↦ a]
+--   := ⟨.app f.fst a.fst, @WTm.app _ _ _ _ _ A.snd B.snd f.snd a.snd⟩
+-- And these convenience functions:
+-- #check wkE
+-- #check wkiE
+-- #check wkpE
+
+-- TODO: Some funky notation (and maybe remove the notation from the -E stuff, it won't be needed now)
+notation δ " ∘ " σ => comp δ σ
+
+#print axioms Con.drop
+#print axioms Con.get
+#print axioms wkn
 
 -- # !
 -- # Everything below this line is VERY out of date!
-
-#exit
-
-#check WTm.app
-#check ESubst.vshift
-/-- `Tm Γ A -> Tm (Γ, B) A` -/
-theorem WSubst.vshift (Γw : WCon Γe) (Aw : WTy Γe Ae) (Bw : WTy (.ext Γe Ae) Be) (tw : WTm Γe Ae te)
-  : WTm (.ext Γe Be) Ae (ESubst.vshift te)
-  := sorry
-    -- match h : te, tw with
-    -- | .var ve, .var vw => by
-    --   rw [ESubst.vshift]
-    --   exact .var (.vs vw)
-    -- | @ETm.app fe ae, @WTm.app Γe .(fe) .(ae) Ae Be Aw' Bw' fw aw => by -- ESubst.vshift (.app f a) ≡ .app (vshift f) (vshift a)
-    --   rw [ESubst.vshift]
-    --   let ih_f := vshift
-    --   -- aesop
-    --   -- have h1 := sorry
-    --   exact @WTm.app (.ext Γe Be) _ _ _ _ _ _ sorry sorry
-    --   done
-    -- | .lam body, .lam bodyw => sorry -- .lam (vshift body)
-    -- | .error, h => sorry
-
-/-- `Subst Γ Δ -> Subst (Γ, A) Δ` -/
-def WSubst.weaken (Γw : WCon Γe) (Δw : WCon Δe) (Aw : WTy Γe Ae) : (σw : WSubst Γe Δe σe) -> WSubst (.ext Γe Ae) Δe (weakenE σe) := sorry
-
-/-- `Subst Γ Γ` -/
-def WSubst.id (Γw : WCon Γe) : WSubst Γe Γe (ESubst.id Γe) := sorry
-
-/-- `Subst (Γ, A) Γ`. This is usually two functions chained together: `wk id`, but we only need this version. -/
-def WSubst.wk (Γw : WCon Γe) (Aw : WTy Γe Ae) : WSubst (.ext Γe Ae) Γe (ESubst.wk Γe) := sorry
-
-/-- `subst1 : Subst Γ (Γ, A) -/
-def WSubst.subst1 (Γw : WCon Γe) (Aw : WTy Γe Ae) : WSubst Γe (.ext Γe Ae) (ESubst.id Γe) := sorry
-
--- theorem substVarW : (vE : EVar) -> (σE : ESubst) -> (tE : ETm) -> W
-
-/-- Remember that `def substTy {Γ Δ : Con} : Ty Δ -> Subst Γ Δ -> Ty Γ` -/
-theorem substTyW {Γe Δe : ECon} {Ae : ETy} (Aw : WTy Δe Ae) {σe : ESubst} (σw : WSubst Γe Δe σe)
-  : WTy Γe (substTyE Ae σe) := sorry
-
-theorem substTmW {Γe Δe : ECon} {te : ETm} (tw : WTm Δe Ae te) {σe : ESubst} (σw : WSubst Γe Δe σe)
-  : WTm Γe (substTyE Ae σe) (substTmE te σe) := sorry
-
-theorem wkW (Γw : WCon Γe) (Aw : WTy Γe Ae) : WSubst (.ext Γe Ae) Γe (ESubst.wk Γe) := sorry
-
-theorem subst1W (Γw : WCon Γe) (Aw : WTy Γe Ae) (tw : WTm Γe Ae te) : WSubst Γe (ECon.ext Γe Ae) (ESubst.subst1 Γe te) := sorry -- maybe? very wild guess
-
-section Hooray
-  def Con : Type _ := @PSigma ECon WCon
-  def Ty (Γ : Con) : Type _ := @PSigma ETy (WTy Γ.fst)
-  def Var (Γ : Con) (A : Ty Γ) : Type _ := @PSigma EVar (WVar Γ.fst A.fst)
-  def Tm (Γ : Con) (A : Ty Γ) : Type _ := @PSigma ETm (WTm Γ.fst A.fst)
-  def Subst (Γ : Con) (Δ : Con) : Type _ := @PSigma ESubst (WSubst Γ.fst Δ.fst)
-
-  def Con.nil : Con := ⟨.nil, .nil⟩
-  def Con.ext (Γ : Con) (A : Ty Γ) : Con := ⟨.ext Γ.fst A.fst, .ext Γ.snd A.snd⟩
-
-  def wk : Subst (Con.ext Γ A) Γ := ⟨ESubst.wk Γ.fst, wkW Γ.snd A.snd⟩
-  def substTy {Γ Δ : Con} (A : Ty Δ) (σ : Subst Γ Δ) : Ty Γ := ⟨substTyE A.fst σ.fst, substTyW A.snd σ.snd⟩
-  def substTm {Γ Δ : Con} {A : Ty Δ} (t : Tm Δ A) (σ : Subst Γ Δ) : Tm Γ (substTy A σ) := ⟨substTmE t.fst σ.fst, substTmW t.snd σ.snd⟩
-
-  def Ty.U : Ty Γ := ⟨.U, .U⟩
-  def Ty.El (t : Tm Γ U) : Ty Γ := ⟨.El t.fst, .El t.snd⟩
-  def Ty.Pi (A : Ty Γ) (B : Ty (Con.ext Γ A)) : Ty Γ := ⟨.Pi A.fst B.fst, .Pi A.snd B.snd⟩
-  def Var.vz : Var (Con.ext Γ A) (substTy A wk) := ⟨.vz, .vz⟩
-  def Var.vs (v : Var Γ A) : Var (Con.ext Γ B) (substTy A wk) := ⟨.vs v.fst, .vs v.snd⟩
-
-  def Subst.nil : Subst Γ Con.nil := ⟨.nil, .nil⟩
-  def Subst.cons (δ : Subst Γ Δ) (t : Tm Γ (substTy A δ)) : Subst Γ (Con.ext Δ A) := ⟨.cons δ.fst t.fst, .cons δ.snd t.snd⟩
-
-  def subst1 (t : Tm Γ A) : Subst Γ (Con.ext Γ A) := ⟨ESubst.subst1 Γ.fst t.fst, subst1W Γ.snd A.snd t.snd⟩
-
-  def Tm.app {A : Ty Γ} {B : Ty (Con.ext Γ A)} (f : Tm Γ (Ty.Pi A B)) (a : Tm Γ A) : Tm Γ (substTy B (subst1 a)) -- Tm Γ B[Var.vz ↦ a]
-    := ⟨.app f.fst a.fst, @WTm.app _ _ _ _ _ A.snd B.snd f.snd a.snd⟩
-  -- def Tm.lam
-  -- def Tm.var
-end Hooray
-
-def weaken : Subst Γ Δ -> Subst (.ext Γ A) Δ := sorry
-
-/-
-  def vshiftE (Γ : ECon) (A X : ETy) : ETm -> ETm
-  | .var Γ A v => -- `v : Var Γ A`   ⊢   `Tm (Γ, X) (substTy A wk)`
-    .var (.ext Γ X)
-      -- `.var (Γ, X) : (A : Ty (Γ, X)) -> Var (Γ, X) A -> Tm (Γ, X) A`
-      (substTyE A (weakenE Γ Γ X (idE Γ))) -- `weaken Subst.id : Subst (Γ, X) Γ`    `substTyE A wk : Ty (Γ, X)`
-      -- `.var (Γ, X) (substTy A wk) : Var (Γ, X) (substTy A wk) -> Tm (Γ, X) (substTy A wk)`
-      (.vs Γ A X -- `.vs Γ A X : Var Γ A -> Var (Γ, X) (substTy A wk)`
-        v
-      )
-  -- Reminder: `Tm.app {Γ} : {A : Ty Γ} -> {B : Ty (Γ, A)} -> (f : Tm Γ (Pi A B)) -> (a : Tm Γ A) -> Tm Γ B[Var.vz ↦ a]`
--- ! | .app Γ A B f a => -- Have   `A : Ty Γ`    `B : Ty (Γ, A)`   `f : Tm Γ (Pi A B)`    `a : Tm Γ A`      expecting `Tm (Γ, X) B[a][wk]`       note that `B[a] : Ty Γ`, and then `B[a][wk] : Ty (Γ, X)`
-    .app (.ext Γ X) -- `app (Γ, X) : (A : Ty (Γ, X)) -> {B : Ty (Γ, X, A)} -> (f : Tm (Γ, X) (Pi A B)) -> (a : Tm (Γ, X) A) -> Tm (Γ, X) B[Var.vz ↦ a]`
-      (substTyE A (weakenE Γ Γ X (idE Γ)))
-      -- `app (Γ, X) A[wk] : {B : Ty (Γ, X, A[wk])} -> (f : Tm (Γ, X) (Pi A[wk] B)) -> (a : Tm (Γ, X) A[wk]) -> Tm (Γ, X) B[Var.vz ↦ a]`
-
-    --   (vshiftE Γ (.Pi Γ A B) B f) -- f : Tm Γ (Pi _ _)
-    --   (vshiftE Γ A B a) -- a : Tm Γ A
-  | .lam Γ A B body =>
-    .lam (.ext Γ B) A B (vshiftE body)
-  | .error => .error
-
--/
-#check vshiftE
-def vshift {Γ : Con} {A X : Ty Γ} : Tm Γ A -> Tm (.ext Γ X) (substTy A wk)
-| ⟨.var .., w⟩ => by
-  have v : Var Γ A := sorry
-  have goal : Tm (.ext Γ X) (substTy A wk) := sorry -- Tm.var
-  sorry
-| ⟨.app .., w⟩ =>
-  have B : Ty (.ext Γ A) := sorry -- from pattern matching
-  have f : Tm Γ (.Pi A B) := sorry -- from pattern matching
-  have a : Tm Γ A := sorry -- from pattern matching
-  -- unify Γ with `Γ` (because of pattern matching)
-  -- unify A with `B[a]` (because of pattern matching)
-
-  let a' : Tm (.ext Γ X) (substTy A wk) := vshift a
-  let f' : Tm (.ext Γ X) (.Pi (substTy A wk) B) := sorry
-
-  have goal : Tm (.ext Γ X) (substTy (substTy B (subst1 a)) wk) := by -- expected `Tm (Γ, X) B[a][wk]`, note that `B[a] : Ty Γ`, and then `B[a][wk] : Ty (Γ, X)`
-    have asdf := @Tm.app (.ext Γ X) (substTy A wk)
-
-    done
-  sorry
-| ⟨.lam .., w⟩ => sorry
-| ⟨.error, _⟩ => sorry
-
--- def
-
 
 #exit
 
@@ -740,7 +574,7 @@ variable (appM : {Γ : Con} -> (ΓM : ConM Γ) ->
 
 set_option pp.proofs.threshold 5
 mutual
-  def Tm.rec' {ΓM : ConM Γ} {AM : TyM ΓM A} : (te : ETm) -> (tw : WTm Γ.fst A.fst te) -> TmM ΓM AM ⟨te, tw⟩
+  def Tm.rec' {ΓM : ConM Γ} {AM : TyM ΓM A} : (te : TmE) -> (tw : WTm Γ.fst A.fst te) -> TmM ΓM AM ⟨te, tw⟩
   | .var v, w => sorry
   | .app fe ae, w => by
     rename Ty Γ => B_subst_a -- `B_subst_a ≡ B[Var.vz ↦ a]`
@@ -756,22 +590,22 @@ mutual
   | .lam body, w => sorry
   | .error, w => sorry
 
-  def Con.rec' : (Γe : ECon) -> (Γw : WCon Γe) -> ConM ⟨Γe, Γw⟩
+  def Con.rec' : (Γe : ConE) -> (Γw : WCon Γe) -> ConM ⟨Γe, Γw⟩
   | .nil, w => nilM
   | .ext Γe Ae, w =>
     let ih_Γ := Con.rec' Γe (let .ext Γw _ := w; Γw)
     let ih_A := Ty.rec' ih_Γ Ae (let .ext _ Aw := w; Aw)
     extM ih_Γ ih_A
 
-  def Ty.rec' {Γ : Con} (ΓM : ConM Γ) : (Ae : ETy) -> (Aw : WTy Γ.fst Ae) -> TyM ΓM ⟨Ae, Aw⟩
-  | ETy.U, w => sorry
+  def Ty.rec' {Γ : Con} (ΓM : ConM Γ) : (Ae : TyE) -> (Aw : WTy Γ.fst Ae) -> TyM ΓM ⟨Ae, Aw⟩
+  | TyE.U, w => sorry
   | .El t, w => sorry
   | .Pi Ae Be, w =>
     let AM : TyM .. := Ty.rec' ΓM Ae (let .Pi Aw Bw := w; Aw)
     let BM : TyM .. := Ty.rec' (extM ΓM AM) Be (let .Pi Aw Bw := w; Bw) -- how the fuck does lean just... accept termination for this? with no massaging? wow
     PiM ΓM AM BM
 
-  def Subst.rec' {Γ : Con} (ΓM : ConM Γ) {Δ : Con} (ΔM : ConM Δ) : (σe : ESubst) -> (σw : WSubst Γ.fst Δ.fst σe) -> SubstM ΓM ΔM ⟨σe, σw⟩
+  def Subst.rec' {Γ : Con} (ΓM : ConM Γ) {Δ : Con} (ΔM : ConM Δ) : (σe : SubstE) -> (σw : WSubst Γ.fst Δ.fst σe) -> SubstM ΓM ΔM ⟨σe, σw⟩
   | .nil, w => sorry -- substNilM ΓM --(let .nil := w; sorry)
   | .cons σe te, w => sorry
 end
